Remove _typeinf, _typecheck

TypeChecker.v
@@ -11,44 +11,44 @@ Import ListNotations.
 Require Import AST.
 Require Import Maps.
 
-Inductive _typecheck : environment -> t_expr -> type -> Prop :=
+Inductive typecheck : environment -> t_expr -> type -> Prop :=
   (* t_Num *)
   (* t_Bool *)
   (* t_Var *)
   | TC_Num: forall env n,
-    _typecheck env (t_Num n) TNum
+    typecheck env (t_Num n) TNum
   | TC_Bool: forall env b,
-    _typecheck env (t_Bool b) TBool
+    typecheck env (t_Bool b) TBool
   | TC_Var: forall env x T,
-    env x = Some T -> _typecheck env (t_Var x) T
+    env x = Some T -> typecheck env (t_Var x) T
 
   (* t_If *)
   | TC_If: forall env c e1 e2 T,
-    _typecheck env c TBool ->
-    _typecheck env e1 T ->
-    _typecheck env e2 T ->
-    _typecheck env (t_If c e1 e2) T
+    typecheck env c TBool ->
+    typecheck env e1 T ->
+    typecheck env e2 T ->
+    typecheck env (t_If c e1 e2) T
 
   (* t_Fun *)
   | TC_Fun: forall env x x_T e e_T,
-    _typecheck (update env x x_T) e e_T ->
-    _typecheck env (t_Fun x x_T e) (TFun x_T e_T)
+    typecheck (update env x x_T) e e_T ->
+    typecheck env (t_Fun x x_T e) (TFun x_T e_T)
 
   (* t_Call *)
   | TC_Call: forall env f e e_T T,
-    _typecheck env f (TFun e_T T) ->
-    _typecheck env e e_T ->
-    _typecheck env (t_Call f e) T
+    typecheck env f (TFun e_T T) ->
+    typecheck env e e_T ->
+    typecheck env (t_Call f e) T
 
   (* t_Cons *)
   | TC_Cons: forall env hd tl T,
-    _typecheck env hd T ->
-    _typecheck env tl (TList T) ->
-    _typecheck env (t_Cons hd tl) (TList T)
+    typecheck env hd T ->
+    typecheck env tl (TList T) ->
+    typecheck env (t_Cons hd tl) (TList T)
 
   (* t_Nil *)
   | TC_Nil: forall env T,
-    _typecheck env (t_Nil T) (TList T)
+    typecheck env (t_Nil T) (TList T)
 
   (* t_Binop *)
   | TC_Binop_nnn: forall env op e1 e2,
@@ -57,24 +57,22 @@ Inductive _typecheck : environment -> t_expr -> type -> Prop :=
     op = op_Mult \/
     op = op_Div \/
     op = op_Mod ->
-    _typecheck env e1 TNum ->
-    _typecheck env e2 TNum ->
-    _typecheck env (t_Binop op e1 e2) TNum
+    typecheck env e1 TNum ->
+    typecheck env e2 TNum ->
+    typecheck env (t_Binop op e1 e2) TNum
 
   | TC_Binop_nnb: forall env op e1 e2,
     op = op_Eq \/
     op = op_Neq \/
     op = op_Lt \/
     op = op_Gt ->
-    _typecheck env e1 TNum ->
-    _typecheck env e2 TNum ->
-    _typecheck env (t_Binop op e1 e2) TBool
+    typecheck env e1 TNum ->
+    typecheck env e2 TNum ->
+    typecheck env (t_Binop op e1 e2) TBool
 
   | TC_Binop_bbb: forall env op e1 e2,
     op = op_And \/
     op = op_Or ->
-    _typecheck env e1 TBool ->
-    _typecheck env e2 TBool ->
-    _typecheck env (t_Binop op e1 e2) TBool.
-
-Definition typecheck e := _typecheck (@empty type) e.
+    typecheck env e1 TBool ->
+    typecheck env e2 TBool ->
+    typecheck env (t_Binop op e1 e2) TBool.
