TypeInferencer.v
@@ -12,16 +12,16 @@ Require Import AST.
 Require Import Maps.
 
 
-Inductive _typeinf : environment -> nat -> ut_expr -> (nat * type * constraint) % type -> Prop :=
+Inductive typeinf : environment -> nat -> ut_expr -> (nat * type * constraint) % type -> Prop :=
   (* ut_Num *)
   (* ut_Bool *)
   (* ut_Var *)
   | TI_Num: forall env n fv,
-    _typeinf env fv  (ut_Num n) (fv, TNum, [])
+    typeinf env fv  (ut_Num n) (fv, TNum, [])
   | TI_Bool: forall env b fv,
-    _typeinf env fv  (ut_Bool b) (fv, TBool, [])
+    typeinf env fv  (ut_Bool b) (fv, TBool, [])
   | TI_Var: forall env x fv T,
-    env x = Some T -> _typeinf env fv (ut_Var x) (fv, T, [])
+    env x = Some T -> typeinf env fv (ut_Var x) (fv, T, [])
 
   (* ut_If *)
   | TI_If:
@@ -29,40 +29,40 @@ Inductive _typeinf : environment -> nat -> ut_expr -> (nat * type * constraint) 
       c c_fv c_C c_T
       e1 e1_fv e1_C e1_T
       e2 e2_fv e2_C e2_T,
-    _typeinf env fv c (c_fv, c_T, c_C) ->
-    _typeinf env c_fv  e1 (e1_fv, e1_T, e1_C) ->
-    _typeinf env e1_fv  e2 (e2_fv, e2_T, e2_C) ->
-    _typeinf env fv (ut_If c e1 e2) (e2_fv, e1_T, e2_C ++ e1_C ++ c_C ++ [(e1_T, e2_T); (c_T, TBool)])
+    typeinf env fv c (c_fv, c_T, c_C) ->
+    typeinf env c_fv  e1 (e1_fv, e1_T, e1_C) ->
+    typeinf env e1_fv  e2 (e2_fv, e2_T, e2_C) ->
+    typeinf env fv (ut_If c e1 e2) (e2_fv, e1_T, e2_C ++ e1_C ++ c_C ++ [(e1_T, e2_T); (c_T, TBool)])
 
   (* ut_Fun *)
   | TI_Fun:
     forall env fv
       x e e_fv e_C e_T,
-    _typeinf (update env x (TVar (Id fv))) (fv + 1)  e (e_fv, e_T, e_C) ->
-    _typeinf env fv (ut_Fun x e) (e_fv, (TFun (TVar (Id fv)) e_T), e_C)
+    typeinf (update env x (TVar (Id fv))) (fv + 1)  e (e_fv, e_T, e_C) ->
+    typeinf env fv (ut_Fun x e) (e_fv, (TFun (TVar (Id fv)) e_T), e_C)
 
   (* ut_Call *)
   | TI_Call:
     forall env fv
       f f_fv f_C f_T
       e e_fv e_C e_T,
-    _typeinf env fv f (f_fv, f_T, f_C) ->
-    _typeinf env f_fv e (e_fv, e_T, e_C) ->
-    _typeinf env fv (ut_Call f e) (e_fv + 1, TVar (Id e_fv), e_C ++ f_C ++ [(f_T, TFun e_T (TVar (Id e_fv)))])
+    typeinf env fv f (f_fv, f_T, f_C) ->
+    typeinf env f_fv e (e_fv, e_T, e_C) ->
+    typeinf env fv (ut_Call f e) (e_fv + 1, TVar (Id e_fv), e_C ++ f_C ++ [(f_T, TFun e_T (TVar (Id e_fv)))])
 
   (* ut_Cons *)
   | TI_Cons:
     forall env fv
       hd hd_fv hd_C hd_T
       tl tl_fv tl_C tl_T,
-    _typeinf env fv hd (hd_fv, hd_T, hd_C) ->
-    _typeinf env hd_fv tl (tl_fv, tl_T, tl_C) ->
-    _typeinf env fv (ut_Cons hd tl) (tl_fv, TList hd_T, tl_C ++ hd_C ++ [(tl_T, TList hd_T)])
+    typeinf env fv hd (hd_fv, hd_T, hd_C) ->
+    typeinf env hd_fv tl (tl_fv, tl_T, tl_C) ->
+    typeinf env fv (ut_Cons hd tl) (tl_fv, TList hd_T, tl_C ++ hd_C ++ [(tl_T, TList hd_T)])
 
   (* ut_Nil *)
   | TI_Nil:
     forall env fv,
-    _typeinf env fv ut_Nil (fv + 1, TList (TVar (Id fv)), [])
+    typeinf env fv ut_Nil (fv + 1, TList (TVar (Id fv)), [])
 
   (* ut_Binop *)
   | TI_Binop_nnn:
@@ -74,9 +74,9 @@ Inductive _typeinf : environment -> nat -> ut_expr -> (nat * type * constraint) 
     op = op_Mult \/
     op = op_Div \/
     op = op_Mod ->
-    _typeinf env fv e1 (e1_fv, e1_T, e1_C) ->
-    _typeinf env e1_fv e2 (e2_fv, e2_T, e2_C) ->
-    _typeinf env fv (ut_Binop op e1 e2) (e2_fv, TNum, e2_C++ e1_C ++ [(e2_T, TNum); (e1_T, TNum)])
+    typeinf env fv e1 (e1_fv, e1_T, e1_C) ->
+    typeinf env e1_fv e2 (e2_fv, e2_T, e2_C) ->
+    typeinf env fv (ut_Binop op e1 e2) (e2_fv, TNum, e2_C++ e1_C ++ [(e2_T, TNum); (e1_T, TNum)])
 
   | TI_Binop_nnb:
     forall env fv op
@@ -86,9 +86,9 @@ Inductive _typeinf : environment -> nat -> ut_expr -> (nat * type * constraint) 
     op = op_Neq \/
     op = op_Lt \/
     op = op_Gt ->
-    _typeinf env fv e1 (e1_fv, e1_T, e1_C) ->
-    _typeinf env e1_fv e2 (e2_fv, e2_T, e2_C) ->
-    _typeinf env fv (ut_Binop op e1 e2) (e2_fv, TBool, e2_C++ e1_C ++ [(e2_T, TNum); (e1_T, TNum)])
+    typeinf env fv e1 (e1_fv, e1_T, e1_C) ->
+    typeinf env e1_fv e2 (e2_fv, e2_T, e2_C) ->
+    typeinf env fv (ut_Binop op e1 e2) (e2_fv, TBool, e2_C++ e1_C ++ [(e2_T, TNum); (e1_T, TNum)])
 
   | TI_Binop_bbb:
     forall env fv op
@@ -96,14 +96,10 @@ Inductive _typeinf : environment -> nat -> ut_expr -> (nat * type * constraint) 
       e2 e2_fv e2_C e2_T,
     op = op_And \/
     op = op_Or ->
-    _typeinf env fv e1 (e1_fv, e1_T, e1_C) ->
-    _typeinf env e1_fv e2 (e2_fv, e2_T, e2_C) ->
-    _typeinf env fv (ut_Binop op e1 e2) (e2_fv, TBool, e2_C++ e1_C ++ [(e2_T, TBool); (e1_T, TBool)]).
+    typeinf env fv e1 (e1_fv, e1_T, e1_C) ->
+    typeinf env e1_fv e2 (e2_fv, e2_T, e2_C) ->
+    typeinf env fv (ut_Binop op e1 e2) (e2_fv, TBool, e2_C++ e1_C ++ [(e2_T, TBool); (e1_T, TBool)]).
 
-(* this is ugly *)
-Inductive typeinf : ut_expr -> (type * constraint) % type -> Prop :=
-  | Wrap: forall e n C T,
-    _typeinf (@empty type) 0 e (n, T, C) -> typeinf e (T, C).
 
 Fixpoint occurs (i : id) (t : type) : bool :=
   match t with
