Proofs.v
@@ -10,23 +10,27 @@ Open Scope core_scope.
 Import ListNotations.
 
 Require Import AST.
+Require Import Maps.
 Require Import TypeInferencer.
 Require Import TypeChecker.
 
+(* Main goals *)
 Theorem typeinference_soundness :
   forall (t : t_expr) (T : type)
-    (e : ut_expr) (S : type) (C : constraint),
+    (e : ut_expr) (env : environment) (fv : nat) (S : type) (C : constraint),
+  env = (@empty type) ->
   erase t = e ->
-  typecheck t T ->
-  typeinf e (S, C) ->
+  typecheck env t T ->
+  typeinf env 0 e (fv, S, C) ->
   (exists (s : substitution), solution s C /\ apply s S = T).
 Proof.
 Admitted.
 
 Theorem typeinference_completeness :
-  forall (e : ut_expr) (S : type) (C :constraint) (s : substitution),
-  typeinf e (S, C) ->
+  forall (e : ut_expr) (env : environment) (fv : nat) (S : type) (C :constraint) (s : substitution),
+  env = (@empty type) ->
+  typeinf env 0 e (fv, S, C) ->
   solution s C ->
-  (exists (t : t_expr), erase t = e /\ typecheck t (apply s S)).
+  (exists (t : t_expr), erase t = e /\ typecheck env t (apply s S)).
 Proof.
 Admitted.
